@prefix : <http://schema.org/> .
@prefix rdf: <http://www.w3.org/1999/02/22-rdf-syntax-ns#> .
@prefix rdfs: <http://www.w3.org/2000/01/rdf-schema#> .

:WebAPI a rdfs:Class ;
    rdfs:label "WebAPI" ;
    :category "issue-1423" ;
    :isPartOf <http://pending.schema.org> ;
    :source <https://github.com/schemaorg/schemaorg/issues/1423> ;
    rdfs:comment """An application programming interface accessible over Web/Internet technologies.

The [[documentation]] property gives specific details of the actual endpoint instances, while the [[conformsTo]] property is used to indicate the general standard or specification that the endpoints implement. The [[url]] property indicates a landing page for the API, which is a Web page that can be navigated to in a Web browser to gain access to the API and/or additional information.

      """ ;
    rdfs:subClassOf :Service .

:documentation a rdf:Property ;
    rdfs:label "documentation" ;
    :category "issue-1423" ;
    :domainIncludes :WebAPI ;
    :isPartOf <http://pending.schema.org> ;
    :rangeIncludes :CreativeWork,
        :URL ;
    :source <https://github.com/schemaorg/schemaorg/issues/1423> ;
    rdfs:comment """Human-readable documentation of the services available via the [[WebAPI]], including their operations, parameters etc.

[[endpointDescription]] should be used for machine-readable documentation.
      """ .

:endpointDescription a rdf:Property ;
    rdfs:label "endpointDescription" ;
    :category "issue-1423" ;
    :domainIncludes :WebAPI ;
    :isPartOf <http://pending.schema.org> ;
    :rangeIncludes :CreativeWork ;
    :source <https://github.com/schemaorg/schemaorg/issues/1423> ;
    rdfs:comment """Machine-readable API definition of the services available via the [[WebAPI]], including their operations, parameters etc.

Machine-readable formats include OpenAPI (Swagger) description, an OGC GetCapabilities response WFS, ISO-19142, WMS, ISO-19128, a SPARQL Service Description, an OpenSearch or WSDL20 document, or a Hydra API description. The [[encodingFormat]] property of the [[CreativeWork]] should be used to indicate the use of such formats via their MIME type.

The [[endpointDescription]] property gives specific details of the actual endpoint instances, while the [[conformsTo]] property is used to indicate the general standard or specification that the endpoints implement.
      """ .

:termsOfService a rdf:Property ;
    rdfs:label "termsOfService" ;
    :category "issue-1423" ;
    :domainIncludes :Service ;
    :isPartOf <http://pending.schema.org> ;
    :rangeIncludes :Text,
        :URL ;
    :source <https://github.com/schemaorg/schemaorg/issues/1423> ;
    rdfs:comment "Human-readable terms of service documentation." .

:endpointUrl a rdf:Property ;
    rdfs:label "endpointUrl" ;
    :category "issue-1423" ;
    :domainIncludes :WebAPI ;
    :isPartOf <http://pending.schema.org> ;
    :rangeIncludes :EntryPoint,
        :URL ;
    :source <https://github.com/schemaorg/schemaorg/issues/1423> ;
    rdfs:comment "The root location or primary endpoint of the API." .

:conformsTo a rdf:Property ;
    rdfs:label "conformsTo" ;
    :category "issue-1423" ;
    :domainIncludes :WebAPI ;
    :isPartOf <http://pending.schema.org> ;
    :rangeIncludes :URL ;
    :source <https://github.com/schemaorg/schemaorg/issues/1423> ;
    rdfs:comment "The URL reference of an established standard to which the described API conforms, for example `https://jsonapi.org/format/1.0/`." .

:accessService a rdf:Property ;
    rdfs:label "accessService" ;
    :category "issue-1423" ;
    :domainIncludes :Dataset,
        :DataDownload ;
    :isPartOf <http://pending.schema.org> ;
    :rangeIncludes :WebAPI ;
    :source <https://github.com/schemaorg/schemaorg/issues/1423> ;
    rdfs:comment "An API that provides access to the dataset." .

:apiTransport a rdf:Property ;
    rdfs:label "apiTransport" ;
    :category "issue-1423" ;
    :domainIncludes :WebAPI ;
    :isPartOf <http://pending.schema.org> ;
    :rangeIncludes :Text ;
    :source <https://github.com/schemaorg/schemaorg/issues/1423> ;
    rdfs:comment "The type of transport used for the API, such as `HTTP`, `HTTPS`, `SMTP`, `MQTT`, `WS`, `WSS`, `gRPC`." .

:version a rdf:Property ;
    :domainIncludes :WebAPI .

:license a rdf:Property ;
    :domainIncludes :WebAPI .
