@prefix : <http://schema.org/> .
@prefix rdf: <http://www.w3.org/1999/02/22-rdf-syntax-ns#> .
@prefix rdfs: <http://www.w3.org/2000/01/rdf-schema#> .

# Add support for structured priceType values (https://github.com/schemaorg/schemaorg/issues/2712)

# extend the domain of priceType to include CompoundPriceSpecification
# add PriceTypeEnumeration to the allowed types to support structured values for price types
:priceType 
	:domainIncludes :CompoundPriceSpecification ;
	:rangeIncludes :PriceTypeEnumeration .
	
:PriceTypeEnumeration a rdfs:Class ;
	rdfs:label "PriceTypeEnumeration" ;
	rdfs:subClassOf :Enumeration ;
	:category "issue-2712" ;
	:isPartOf <http://pending.schema.org> ;
	:source <https://github.com/schemaorg/schemaorg/issues/2712> ;
	rdfs:comment "Enumerates different price types, for example list price, invoice price, and sale price." .

:ListPrice a :PriceTypeEnumeration ;
	rdfs:label "ListPrice" ;
	:category "issue-2712" ;
	:isPartOf <http://pending.schema.org> ;
	:source <https://github.com/schemaorg/schemaorg/issues/2712> ;
	rdfs:comment "Represents the list price (the price a product is actually advertised for) of an offered product." .

:SalePrice a :PriceTypeEnumeration ;
	rdfs:label "SalePrice" ;
	:category "issue-2712" ;
	:isPartOf <http://pending.schema.org> ;
	:source <https://github.com/schemaorg/schemaorg/issues/2712> ;
	rdfs:comment "Represents a sale price (usually active for a limited period) of an offered product." .
	
:MSRP a :PriceTypeEnumeration ;
	rdfs:label "MSRP" ;
	:category "issue-2712" ;
	:isPartOf <http://pending.schema.org> ;
	:source <https://github.com/schemaorg/schemaorg/issues/2712> ;
	rdfs:comment """Represents the manufacturer suggested retail price ("MSRP") of an offered product.""" .

:SRP a :PriceTypeEnumeration ;
	rdfs:label "SRP" ;
	:category "issue-2712" ;
	:isPartOf <http://pending.schema.org> ;
	:source <https://github.com/schemaorg/schemaorg/issues/2712> ;
	rdfs:comment """Represents the suggested retail price ("SRP") of an offered product.""" .

:InvoicePrice a :PriceTypeEnumeration ;
	rdfs:label "InvoicePrice" ;
	:category "issue-2712" ;
	:isPartOf <http://pending.schema.org> ;
	:source <https://github.com/schemaorg/schemaorg/issues/2712> ;
	rdfs:comment "Represents the invoice price of an offered product." .
	
:MinimumAdvertisedPrice a :PriceTypeEnumeration ;
	rdfs:label "MinimumAdvertisedPrice" ;
	:category "issue-2712" ;
	:isPartOf <http://pending.schema.org> ;
	:source <https://github.com/schemaorg/schemaorg/issues/2712> ;
	rdfs:comment """Represents the minimum advertised price ("MAP") (as dictated by the manufacturer) of an offered product.""" .
		