@prefix : <http://schema.org/> .
@prefix rdf: <http://www.w3.org/1999/02/22-rdf-syntax-ns#> .
@prefix rdfs: <http://www.w3.org/2000/01/rdf-schema#> .

:SolveMathAction a rdfs:Class ;
    rdfs:label "SolveMathAction" ;
    :category "issue-2740" ;
    :isPartOf <http://pending.schema.org> ;
    :source <https://github.com/schemaorg/schemaorg/issues/2740> ;
    rdfs:comment "The action that takes in a math expression and directs users to a page potentially capable of solving/simplifying that expression." ;
    rdfs:subClassOf :Action .
    
:MathSolver a rdfs:Class ;
    rdfs:label "MathSolver" ;
    :category "issue-2740" ;
    :isPartOf <http://pending.schema.org> ;
    :source <https://github.com/schemaorg/schemaorg/issues/2740> ;
    rdfs:comment "A math solver which is capable of solving a subset of mathematical problems." ;
    rdfs:subClassOf :CreativeWork .
    
:mathExpression a rdf:Property ;
    rdfs:label "mathExpression" ;
    :category "issue-2740" ;
    :domainIncludes :GovernmentService,
        :Legislation ;
    :isPartOf <http://pending.schema.org> ;
    :rangeIncludes :SolveMathAction,
        :Text ;
    :source <https://github.com/schemaorg/schemaorg/issues/2740> ;
    rdfs:comment "A mathematical expression (e.g. “x^2-3x=0”) that may be solved for a specific variable, simplified, or transformed. This can take many formats, e.g. LaTeX, Ascii-Math, or math as you would write with a keyboard." .
